
***
*Solution:*
Since $X_1$ and $X_2$ are independent gamma random variables,
$$ 
\begin{aligned}
			f(x_1, x_2) &= f(x_1) f(x_2) \\
			&= \frac{x_1^{-\frac{1}{2}} e^{-\frac{x_1}{\theta}}}{ \left( \pi \theta \right)^{\frac{1}{2}}} \frac{x_2^{-\frac{1}{2}} e^{-\frac{x_2}{\theta}}}{ \left( \pi \theta \right)^{\frac{1}{2}}} \\
			&= \frac{\left( x_1 x_2 \right)^{-\frac{1}{2}} e^{- \frac{1}{\theta}\left( x_1 + x_2 \right)}}{\pi \theta}, \qquad x_1, x_2 > 0.
\end{aligned} 
$$
Now, let $Y_1 = X_1 + X_2$ and $Y_2 = X_1 - X_2$. Thus,
$$
	X_1 = \frac{Y_1 + Y_2}{2} \qquad X_2 = \frac{Y_1 - Y_2}{2}
$$
and the Jacobian is given by
$$ 
\begin{aligned}
		|J| &= \left| \text{det} \begin{bmatrix} \dfrac{\partial x_1}{\partial y_1} & \dfrac{\partial x_1}{\partial y_2} \\[2ex] \dfrac{\partial x_2}{\partial y_1} & \dfrac{\partial x_2}{\partial y_2} \end{bmatrix} \right| \\
		&=\left| \text{det} \begin{bmatrix} \dfrac{1}{2} & \dfrac{1}{2} \\[2ex] \dfrac{1}{2} & -\dfrac{1}{2} \end{bmatrix}\right| \\
		&= \left| - \frac{1}{2} \right| = \frac{1}{2}.
\end{aligned} 
$$
	
The joint pdf of $Y_1$ and $Y_2$ is thus
$$ 
\begin{aligned}
	g(y_1, y_2) &= \frac{1}{2\pi \theta} \left[ \left( \frac{y_1 + y_2}{2} \right) \left( \frac{y_1 - y_2}{2}\right) \right]^{-\frac{1}{2}} e^{-\frac{1}{\theta} \left(\frac{y_1 + y_2}{2} + \frac{y_1 - y_2}{2} \right)} \\
	&= \frac{1}{\pi\theta} \frac{1}{\sqrt{y_1^2 - y_2^2}} e^{-\frac{y_1}{\theta}}.
	\end{aligned}
$$
```{marginfigure}
\begin{tikzpicture}[scale=0.3]
  \draw[fill = gray!50, draw = white] (2, 2) -- (2, 13) -- (13, 13) -- (13, 2) -- (2, 2);
  \draw [very thick, -latex] (0, 2) -- (13, 2);
  \draw [very thick, -latex] (2, 0) -- (2, 13);
  \node at (13.5, 2) { $X_1$ };
  \node at (2, 13.5) { $X_2$ };
\end{tikzpicture}
```

To determine the support of the new random varibles:
For $y_{1} = x_{1} + x_{2}$ note that $x_{1} > 0$, $x_{2} > 0$, therefore $y_{1} > 0$.
For $y_{2}$ note that 
$$
\begin{aligned}
			& x_1 > 0 \Rightarrow & \frac{y_1 + y_2 }{2} > 0 \Rightarrow & \quad y_2 > - y_1 \\ 
			& x_2 > 0 \Rightarrow & \frac{y_1 - y_2}{2} > 0 \Rightarrow &\quad  y_2 < y_1\\
\end{aligned}
$$
Therfore $y_{1} > 0$ and $- y_{1} < y_{2} < y_{1}$.

```{marginfigure}
\begin{tikzpicture}[scale=0.3]
\draw [fill = gray!50, draw = white] (2,6) -- (8.5, -0.5)arc(-45:45:9.1924) -- (2, 6);

\draw [very thick, -latex] (-1, 6) -- (13, 6);
\draw [very thick, -latex] (2, 0) -- (2, 13);

\draw [thick, dashed,] (0, 4) -- (9, 13);
\draw [thick, dashed,] (0, 8) -- (9,-1);

\node at (13.5, 6) { $Y_1$ };
\node at (2, 13.5) { $Y_2$ };

\node at (6.5,12.5) {$ y_2 = y_1 $}; 
\node at (12, 0) {$ y_2 = -y_1 $}; 
\end{tikzpicture}
```

Clearly, $Y_1$ and $Y_2$ are not independent. The joint distribution cannot be split into 2 separate functions of $y_1$ and $y_2$ alone, AND the ranges depend on each other.

***